compiler/core/Imp/Optim/ImpEJsonOptimizerEngine.v
@@ -1,0 +1,232 @@
+(*
+ * Licensed under the Apache License, Version 2.0 (the "License");
+ * you may not use this file except in compliance with the License.
+ * You may obtain a copy of the License at
+ *
+ * http://www.apache.org/licenses/LICENSE-2.0
+ *
+ * Unless required by applicable law or agreed to in writing, software
+ * distributed under the License is distributed on an "AS IS" BASIS,
+ * WITHOUT WARRANTIES OR CONDITIONS OF ANY KIND, either express or implied.
+ * See the License for the specific language governing permissions and
+ * limitations under the License.
+ *)
+
+(** Imp is a simpl imperative intermediate language. *)
+
+Require Import String.
+Require Import List.
+Require Import Bool.
+Require Import Arith.
+Require Import ZArith.
+Require Import Utils.
+Require Import JsAst.JsNumber.
+Require Import EJsonRuntime.
+Require Import Imp.
+Require Import ImpEJson.
+Require Import ImpEJsonVars.
+Require Import ImpEJsonEval.
+
+Section ImpEJsonOptimizerEngine.
+  Import ListNotations.
+
+  Context {foreign_ejson_model:Set}.
+  Context {fejson:foreign_ejson foreign_ejson_model}.
+  Context {foreign_ejson_runtime_op : Set}.
+  Context {fejruntime:foreign_ejson_runtime foreign_ejson_runtime_op}.
+
+  Section OptimizerEngine.
+
+    (* Rewriting functional for into imperative for loop is now isolated *)
+    Fixpoint imp_ejson_stmt_block_rewrite
+             (fs : imp_stmt -> imp_stmt)
+             (stmt: @imp_ejson_stmt foreign_ejson_model foreign_ejson_runtime_op)
+    : imp_ejson_stmt :=
+      match stmt with
+      | ImpStmtBlock lv ls =>
+        fs (ImpStmtBlock
+              lv (* XXX Could add expr rewrite *)
+              (map (imp_ejson_stmt_block_rewrite fs) ls))
+      | ImpStmtAssign v e =>
+        fs (ImpStmtAssign v e)
+      | ImpStmtFor v e s =>
+        fs (ImpStmtFor v e
+                       (imp_ejson_stmt_block_rewrite fs s))
+      | ImpStmtForRange v e1 e2 s =>
+        fs (ImpStmtForRange v e1 e2
+                            (imp_ejson_stmt_block_rewrite fs s))
+      | ImpStmtIf e s1 s2 =>
+        fs (ImpStmtIf e
+                      (imp_ejson_stmt_block_rewrite fs s1)
+                      (imp_ejson_stmt_block_rewrite fs s2))
+      end.
+
+    Definition imp_ejson_function_block_rewrite
+               (fs : imp_stmt -> imp_stmt)
+               (f:imp_function) : imp_function :=
+      match f with
+      | ImpFun v1 s v2 =>
+        ImpFun v1 (imp_ejson_stmt_block_rewrite fs s) v2
+      end.
+    Definition imp_ejson_block_rewrite
+               (fs : imp_stmt -> imp_stmt)
+               (q:imp_ejson) : imp_ejson :=
+      match q with
+      | ImpLib l =>
+        ImpLib (map (fun xy => (fst xy, imp_ejson_function_block_rewrite fs (snd xy))) l)
+      end.
+  End OptimizerEngine.
+
+  Section CorrectnessOptimizerEngine.
+    Lemma imp_ejson_function_stmt_rewrite_correct
+          (fs : imp_stmt -> imp_stmt)
+          h (j:pd_jbindings) (s:imp_ejson_stmt) :
+      (forall s0, forall j0, imp_ejson_stmt_eval h s0 j0 = imp_ejson_stmt_eval h (fs s0) j0) ->
+      imp_ejson_stmt_eval h s j = imp_ejson_stmt_eval h (imp_ejson_stmt_block_rewrite fs s) j.
+    Proof.
+      revert j.
+      induction s; intros; simpl in *.
+      - rewrite <- H0; simpl.
+        generalize (@ImpEval.imp_decls_eval (@imp_ejson_model foreign_ejson_model)
+             (@imp_ejson_constant foreign_ejson_model) imp_ejson_op
+             (@imp_ejson_runtime_op foreign_ejson_runtime_op)
+             (@imp_ejson_model_normalize foreign_ejson_model)
+             (@imp_ejson_runtime_eval foreign_ejson_model fejson foreign_ejson_runtime_op
+                fejruntime h) (@imp_ejson_op_eval foreign_ejson_model) j el); intros.
+        induction el; intros; simpl in *; try reflexivity.
+        + destruct o; intros; simpl; try reflexivity.
+          generalize (Some p).
+          induction sl; intros; simpl in *; try reflexivity.
+          inversion H; clear H; subst.
+          destruct o; simpl; try reflexivity.
+          * rewrite IHsl; clear IHsl; [|assumption].
+            assert (imp_ejson_stmt_eval h a p0
+                    = imp_ejson_stmt_eval h (imp_ejson_stmt_block_rewrite fs a) p0) by
+                apply (H3 p0 H0).
+            rewrite H; reflexivity.
+          * rewrite IHsl; clear IHsl; [reflexivity|assumption].
+        + rewrite IHel; reflexivity.
+      - rewrite <- H; simpl; reflexivity.
+      - rewrite <- H; simpl.
+        destruct (@ImpEval.imp_expr_eval (@imp_ejson_model foreign_ejson_model)
+        (@imp_ejson_constant foreign_ejson_model) imp_ejson_op
+        (@imp_ejson_runtime_op foreign_ejson_runtime_op)
+        (@imp_ejson_model_normalize foreign_ejson_model)
+        (@imp_ejson_runtime_eval foreign_ejson_model fejson foreign_ejson_runtime_op fejruntime h)
+        (@imp_ejson_op_eval foreign_ejson_model) j e); try reflexivity.
+        destruct (imp_ejson_model_to_list i); try reflexivity.
+        revert j.
+        induction l; intros; try reflexivity.
+        rewrite <- IHs; [|assumption].
+        destruct (@imp_ejson_stmt_eval foreign_ejson_model fejson foreign_ejson_runtime_op fejruntime h s
+        (@cons (prod var (option (@imp_ejson_model foreign_ejson_model)))
+           (@pair var (option (@imp_ejson_model foreign_ejson_model)) v
+                  (@Some (@imp_ejson_model foreign_ejson_model) a)) j)); try reflexivity.
+        destruct p; try reflexivity.
+        apply IHl.
+      - rewrite <- H; simpl.
+        destruct (@olift (@imp_ejson_model foreign_ejson_model) Z (@imp_ejson_model_to_Z foreign_ejson_model)
+        (@ImpEval.imp_expr_eval (@imp_ejson_model foreign_ejson_model)
+           (@imp_ejson_constant foreign_ejson_model) imp_ejson_op
+           (@imp_ejson_runtime_op foreign_ejson_runtime_op)
+           (@imp_ejson_model_normalize foreign_ejson_model)
+           (@imp_ejson_runtime_eval foreign_ejson_model fejson foreign_ejson_runtime_op fejruntime
+                                    h) (@imp_ejson_op_eval foreign_ejson_model) j e1)); try reflexivity.
+        destruct (@olift (@imp_ejson_model foreign_ejson_model) Z (@imp_ejson_model_to_Z foreign_ejson_model)
+        (@ImpEval.imp_expr_eval (@imp_ejson_model foreign_ejson_model)
+           (@imp_ejson_constant foreign_ejson_model) imp_ejson_op
+           (@imp_ejson_runtime_op foreign_ejson_runtime_op)
+           (@imp_ejson_model_normalize foreign_ejson_model)
+           (@imp_ejson_runtime_eval foreign_ejson_model fejson foreign_ejson_runtime_op fejruntime
+                                    h) (@imp_ejson_op_eval foreign_ejson_model) j e2)); try reflexivity.
+        generalize (ImpEval.nb_iter z z0); clear z0; intros.
+        revert z j.
+        induction n; intros; try reflexivity.
+        rewrite IHs; clear IHs; [|assumption].
+        destruct (@imp_ejson_stmt_eval foreign_ejson_model fejson foreign_ejson_runtime_op fejruntime h
+        (imp_ejson_stmt_block_rewrite fs s)
+        (@cons (prod var (option (@imp_ejson_model foreign_ejson_model)))
+           (@pair var (option (@imp_ejson_model foreign_ejson_model)) v
+              (@Some (@imp_ejson_model foreign_ejson_model)
+                     (@imp_ejson_Z_to_data foreign_ejson_model z))) j)); try reflexivity.
+        destruct p; try reflexivity.
+        apply IHn.
+      - rewrite <- H; simpl.
+        destruct (@ImpEval.imp_expr_eval (@imp_ejson_model foreign_ejson_model)
+        (@imp_ejson_constant foreign_ejson_model) imp_ejson_op
+        (@imp_ejson_runtime_op foreign_ejson_runtime_op)
+        (@imp_ejson_model_normalize foreign_ejson_model)
+        (@imp_ejson_runtime_eval foreign_ejson_model fejson foreign_ejson_runtime_op fejruntime h)
+        (@imp_ejson_op_eval foreign_ejson_model) j e); try reflexivity.
+        destruct (imp_ejson_model_to_bool i); try reflexivity.
+        destruct b; auto.
+    Qed.
+
+    Lemma imp_ejson_function_block_rewrite_correct
+          (fs : imp_stmt -> imp_stmt)
+          h (j:ejson) (f:imp_ejson_function) :
+      (forall s0, forall j0, imp_ejson_stmt_eval h s0 j0 = imp_ejson_stmt_eval h (fs s0) j0) ->
+      imp_ejson_function_eval h f j = imp_ejson_function_eval h (imp_ejson_function_block_rewrite fs f) j.
+    Proof.
+      intros; destruct f. simpl.
+      assert (imp_ejson_stmt_eval h i [(v0, None); (v, Some j)]
+              = imp_ejson_stmt_eval h (imp_ejson_stmt_block_rewrite fs i) [(v0, None); (v, Some j)])
+        by (apply (imp_ejson_function_stmt_rewrite_correct fs); assumption).
+      unfold imp_ejson_stmt_eval in H0; simpl in *.
+      assert (@ImpEval.imp_stmt_eval (@imp_ejson_model foreign_ejson_model)
+           (@imp_ejson_constant foreign_ejson_model) imp_ejson_op
+           (@imp_ejson_runtime_op foreign_ejson_runtime_op)
+           (@imp_ejson_model_normalize foreign_ejson_model)
+           (@imp_ejson_model_to_bool foreign_ejson_model)
+           (@imp_ejson_model_to_Z foreign_ejson_model)
+           (@imp_ejson_model_to_list foreign_ejson_model)
+           (@imp_ejson_Z_to_data foreign_ejson_model)
+           (@imp_ejson_runtime_eval foreign_ejson_model fejson foreign_ejson_runtime_op fejruntime
+              h) (@imp_ejson_op_eval foreign_ejson_model) i
+           (@cons (prod var (option (@ejson foreign_ejson_model)))
+              (@pair var (option (@ejson foreign_ejson_model)) v0
+                 (@None (@ejson foreign_ejson_model)))
+              (@cons (prod var (option (@ejson foreign_ejson_model)))
+                 (@pair var (option (@ejson foreign_ejson_model)) v
+                    (@Some (@ejson foreign_ejson_model) j))
+                 (@nil (prod var (option (@ejson foreign_ejson_model))))))
+           = @ImpEval.imp_stmt_eval (@imp_ejson_model foreign_ejson_model)
+        (@imp_ejson_constant foreign_ejson_model) imp_ejson_op
+        (@imp_ejson_runtime_op foreign_ejson_runtime_op)
+        (@imp_ejson_model_normalize foreign_ejson_model)
+        (@imp_ejson_model_to_bool foreign_ejson_model) (@imp_ejson_model_to_Z foreign_ejson_model)
+        (@imp_ejson_model_to_list foreign_ejson_model) (@imp_ejson_Z_to_data foreign_ejson_model)
+        (@imp_ejson_runtime_eval foreign_ejson_model fejson foreign_ejson_runtime_op fejruntime h)
+        (@imp_ejson_op_eval foreign_ejson_model) i
+        (@cons (prod var (option (@imp_ejson_model foreign_ejson_model)))
+           (@pair var (option (@imp_ejson_model foreign_ejson_model)) v0
+              (@None (@imp_ejson_model foreign_ejson_model)))
+           (@cons (prod var (option (@imp_ejson_model foreign_ejson_model)))
+              (@pair var (option (@imp_ejson_model foreign_ejson_model)) v
+                 (@Some (@imp_ejson_model foreign_ejson_model) j))
+              (@nil (prod var (option (@imp_ejson_model foreign_ejson_model))))))) by reflexivity.
+      rewrite H1 in H0.
+      rewrite H0; reflexivity.
+    Qed.
+
+    Lemma imp_ejson_block_rewrite_correct
+          (fs : imp_stmt -> imp_stmt)
+          h (j : ejson) (q:imp_ejson) :
+      (forall s0, forall j0, imp_ejson_stmt_eval h s0 j0 = imp_ejson_stmt_eval h (fs s0) j0) ->
+      imp_ejson_eval h q j =
+      imp_ejson_eval h (imp_ejson_block_rewrite fs q) j.
+    Proof.
+      induction q; simpl; intros.
+      destruct l; simpl; intros; [reflexivity|].
+      destruct p; simpl.
+      destruct l; simpl; [|reflexivity].
+      assert (imp_ejson_function_eval h i j
+              = imp_ejson_function_eval h (imp_ejson_function_block_rewrite fs i) j)
+        by (apply imp_ejson_function_block_rewrite_correct; assumption).
+      simpl in H0.
+      unfold imp_ejson_function_eval in H0.
+      rewrite H0; reflexivity.
+    Qed.
+  End CorrectnessOptimizerEngine.
+
+End ImpEJsonOptimizerEngine.
